Slight refactor of mk_blank_tree

fstar/MLS.TreeCommon.Lemmas.fst
@@ -1,8 +1,9 @@
 module MLS.TreeCommon.Lemmas
 
+open MLS.Tree
 open MLS.TreeCommon
 
-#set-options "--fuel 0 --ifuel 0"
+#set-options "--fuel 1 --ifuel 1"
 
 #push-options "--ifuel 2 --fuel 2"
 val mem_insert_sorted: #a:eqtype{a `subtype_of` int} -> x:a -> l:list a -> elem:a -> Lemma
@@ -16,3 +17,14 @@ let rec mem_insert_sorted x l elem =
     else if x = y then ()
     else mem_insert_sorted x (z::t) elem
 #pop-options
+
+val find_empty_leaf_mk_blank_tree: #leaf_t:Type -> #node_t:Type -> l:nat -> i:tree_index l -> Lemma
+  (Some? (find_empty_leaf (mk_blank_tree #leaf_t #node_t l i)))
+let rec find_empty_leaf_mk_blank_tree #leaf_t #node_t l i =
+  if l = 0 then ()
+  else find_empty_leaf_mk_blank_tree #leaf_t #node_t (l-1) (left_index i)
+
+val find_empty_leaf_tree_extend: #leaf_t:Type -> #node_t:Type -> #l:nat -> t:tree (option leaf_t) (option node_t) l 0 -> Lemma
+  (Some? (find_empty_leaf (tree_extend t)))
+let find_empty_leaf_tree_extend #leaf_t #node_t #l t =
+  find_empty_leaf_mk_blank_tree #leaf_t #node_t l (right_index #(l+1) 0)
